theories/Handlers/Storage.v
@@ -78,6 +78,7 @@ Section storage_handler.
       h_initial := stor.new;
       h_spawn _ _ := id;
       h_spawn_covariance _ _ _ _ H := H;
+      h_spawn_commutativity := ltac:(sauto);
       h_terminate _ := id_mfun;
     |}.
 End storage_handler.
