README.md
@@ -1,4 +1,0 @@
-# SLOT
-[![coqchk](https://github.com/libtx/SLOT/actions/workflows/coqchk.yml/badge.svg?branch=master)](https://github.com/libtx/SLOT/actions/workflows/coqchk.yml)
-
-Under construction
